Sequences/DataSizes.dfy
@@ -4,10 +4,16 @@ module DataSizes {
 
   import opened Power2
 
-  predicate is_bit(b: int)  { 0 <= b < 2 }
-  predicate is_byte(b: int) { 0 <= b < 256 }
-  predicate word_16(x: int) { 0 <= x < 0x10000 }
-  predicate word_32(x: int) { 0 <= x < power2(32) }
-  predicate is_word(w: int) { word_32(w) }
+  const BIT:      int := power2(1)
+  const BYTE:     int := power2(8)
+  const WORD_16:  int := power2(16)
+  const WORD_32:  int := power2(32)
+  const WORD_64:  int := power2(64)
+
+  predicate is_bit(x: int)      { 0 <= x < BIT }
+  predicate is_byte(x: int)     { 0 <= x < BYTE }
+  predicate is_word_16(x: int)  { 0 <= x < WORD_16 }
+  predicate is_word_32(x: int)  { 0 <= x < WORD_32 }
+  predicate is_word_64(x: int)  { 0 <= x < WORD_64 }
 
 }
